wrong path; some refactoring

TAPLFormalization/02-lambda/Semantics.lean
@@ -1,6 +1,8 @@
 import TAPLFormalization.«02-lambda».AST
 import TAPLFormalization.«01-peano».Common
 
+import Lean.Elab.App
+
 def addDepth (k : ℕ) : IndexedTerm → IndexedTerm
   | .freeV x => .freeV x
   | .boundV n => .boundV (n+k)
@@ -23,7 +25,8 @@ structure Semantics (T : Type u) where
 
 structure DeterministicSemantics (T : Type u) extends Semantics T where
   next : T → Option T
-  next_none_iff_isNF : next t = none ↔ isNF t
+  deterministic : SmallStep t₁ t₂ ↔ next t₁ = .some t₂
+  isNF_iff_no_step : isNF t ↔ ¬(∃ t', SmallStep t t')
 
 def Semantics.SmallSteps (s : Semantics T) : T → T → Prop := ReflTransGen' s.SmallStep
 def DeterministicSemantics.next_or_id (s : DeterministicSemantics T) (t : T) : T := (s.next t).elim t id
@@ -67,7 +70,7 @@ def NormalOrder : Semantics IndexedTerm where
 namespace CN
   inductive SmallStep : IndexedTerm → IndexedTerm → Prop
     | appBody : SmallStep t₁ t₁' → SmallStep (.app t₁ t₂) (.app t₁' t₂)
-    | appAbs : SmallStep (.app (.abs t₁) t₂) (subst t₂ t₁)
+    | appAbs : (s = subst t₂ t₁) → SmallStep (.app (.abs t₁) t₂) s
 
   inductive Neutral : IndexedTerm → Prop
     | freeV : Neutral (.freeV x)
@@ -77,16 +80,61 @@ namespace CN
   inductive isNF : IndexedTerm → Prop
     | neutral : Neutral t → isNF t
     | abs : isNF (.abs t)
+
+  lemma isNF_iff_no_step : isNF t ↔ ¬(∃ t', SmallStep t t') := by
+    constructor
+    · intro t_nf ⟨t', st⟩
+      cases t_nf with
+      | neutral t_ne =>
+        induction t_ne generalizing t' <;> cases st
+        · grind
+        · contradiction
+      | abs => cases st
+    · intro no_st
+      induction t with
+      | freeV => repeat constructor
+      | boundV => repeat constructor
+      | app body arg body_ih arg_ih =>
+        constructor
+        let body_nf := by
+          apply body_ih
+          intro ⟨body', body_st⟩
+          apply no_st
+          exact ⟨body'.app arg, .appBody body_st⟩
+        apply Neutral.app
+        cases body <;> try grind [isNF, Neutral, subst]
+        cases no_st ⟨subst arg _, SmallStep.appAbs rfl⟩
+      | abs body ih => apply isNF.abs
+
+  mutual
+    def next_app : IndexedTerm → IndexedTerm → Option IndexedTerm
+      | .abs t₁, t₂ => subst t₂ t₁
+      | t₁, t₂ => (.app · t₂) <$> (next t₁)
+
+    def next : IndexedTerm → Option IndexedTerm
+      | .freeV _ => none
+      | .boundV _ => none
+      | .abs _ => none
+      | .app t₁ t₂ => next_app t₁ t₂
+  end
+
+  lemma smallStep_deterministic : SmallStep t₁ t₂ ↔ next t₁ = .some t₂ := by
+    constructor
+    · intro st
+      induction st <;> rw [next, next_app] <;> grind [next]
+    · intro next_eq
+      induction t₁ generalizing t₂ <;> (rw [next] at next_eq; try contradiction)
+      case app body arg body_ih arg_ih =>
+        fun_cases next_app <;> rw [next_app] at next_eq <;> try assumption
+        all_goals grind [Option.map_eq_some_iff, SmallStep]
 end CN
 
-def CallByName : Semantics IndexedTerm where
+def CallByName : DeterministicSemantics IndexedTerm where
   SmallStep := CN.SmallStep
   isNF := CN.isNF
-
-theorem CallByName.isNF_iff_no_step : CallByName.isNF t ↔ ¬(∃ t', CallByName.SmallStep t t') := by
-  constructor
-  · sorry
-  · sorry
+  next := CN.next
+  deterministic := CN.smallStep_deterministic
+  isNF_iff_no_step := CN.isNF_iff_no_step
 
 namespace CV
   inductive SmallStep : IndexedTerm → IndexedTerm → Prop
@@ -94,17 +142,76 @@ namespace CV
     | appArg : SmallStep t₂ t₂' → SmallStep (.app (.abs t₁) t₂) (.app (.abs t₁) t₂')
     | appAbs : (s = subst (.abs t₂) t₁) → SmallStep (.app (.abs t₁) (.abs t₂)) s
 
-  abbrev SmallSteps := ReflTransGen' SmallStep
+  mutual
+    inductive Neutral : IndexedTerm → Prop
+      | freeV : Neutral (.freeV x)
+      | boundV : Neutral (.boundV n)
+      | appNeutral : Neutral t₁ → Neutral (.app t₁ t₂)
+      | appAbs : Neutral t₂ → Neutral (.app (.abs t₁) t₂)
 
-  def next : IndexedTerm → Option IndexedTerm
-    | .freeV _ => none
-    | .boundV _ => none
-    | .abs _ => none
-    | .app (.abs t₁) (.abs t₂) => subst (.abs t₂) t₁
-    | .app (.abs t₁) t₂ => (.app (.abs t₁)) <$> (next t₂)
-    | .app t₁ t₂ => (.app · t₂) <$> (next t₁)
+    inductive isNF : IndexedTerm → Prop
+      | neutral : Neutral t → isNF t
+      | abs : isNF (.abs t)
+  end
 
-  def next_or_id (t : IndexedTerm) : IndexedTerm := (next t).elim t id
+  lemma isNF_iff_no_step : isNF t ↔ ¬(∃ t', SmallStep t t') := by
+    constructor
+    · apply isNF.rec
+      case motive_1 => exact fun t t_ne => ¬∃ t', SmallStep t t'
+      all_goals grind [SmallStep, Neutral]
+    · intro no_st
+      induction t <;> try grind [isNF, Neutral, SmallStep, subst]
+      case app body arg body_ih arg_ih =>
+        let body_nf : isNF body := by
+          apply body_ih
+          intro ⟨body', body_st⟩
+          exact no_st ⟨_, .appBody body_st⟩
+        constructor
+        cases body_nf
+        · constructor
+          assumption
+        · apply Neutral.appAbs
+          let arg_nf : isNF arg := by
+            rename_i t
+            apply arg_ih
+            intro ⟨arg', arg_st⟩
+            apply no_st ⟨_, .appArg arg_st⟩
+          cases arg_nf
+          · assumption
+          · cases no_st ⟨_, .appAbs rfl⟩
 
-  def getNF (gas : ℕ) (t : IndexedTerm) : IndexedTerm := gas.repeat next_or_id t
+  mutual
+    def next_app (t₁ : IndexedTerm) (t₂ : IndexedTerm) : Option IndexedTerm := match t₁, t₂ with
+      | .abs t₁, .abs t₂ => subst (.abs t₂) t₁
+      | .abs t₁, t₂ => (.app (.abs t₁)) <$> (next t₂)
+      | t₁, t₂ => (.app · t₂) <$> (next t₁)
+    termination_by (sizeOf t₁ + sizeOf t₂, 0)
+    decreasing_by
+      constructor
+      all_goals grind [IndexedTerm, SizeOf.sizeOf, IndexedTerm._sizeOf_1]
+
+    def next (t : IndexedTerm) : Option IndexedTerm := match t with
+      | .freeV _ => none
+      | .boundV _ => none
+      | .abs _ => none
+      | .app t₁ t₂ => next_app t₁ t₂
+    termination_by (sizeOf t, 1)
+  end
+
+  lemma smallStep_deterministic : SmallStep t₁ t₂ ↔ next t₁ = .some t₂ := by
+  constructor
+  · intro st
+    induction st <;> rw [next, next_app] <;> try grind [next]
+  · intro next_eq
+    induction t₁ generalizing t₂ <;> (rw [next] at next_eq; try contradiction)
+    case app body arg body_ih arg_ih =>
+      fun_cases next_app <;> rw [next_app] at next_eq <;> try assumption
+      all_goals grind [Option.map_eq_some_iff, SmallStep]
 end CV
+
+def CallByValue : DeterministicSemantics IndexedTerm where
+  SmallStep := CV.SmallStep
+  isNF := CV.isNF
+  next := CV.next
+  deterministic := CV.smallStep_deterministic
+  isNF_iff_no_step := CV.isNF_iff_no_step
