TAPLFormalization/01-peano/BigStep.lean
@@ -2,80 +2,82 @@ import TAPLFormalization.«01-peano».AST
 import TAPLFormalization.«01-peano».Semantics
 import TAPLFormalization.«01-peano».SemanticsTheorems
 
-inductive BigStep : Term → Term → Prop where
-  | value : v.IsValue → BigStep v v
-  | ifTrue : v.IsValue → BigStep t₁ .trueV → BigStep t₂ v
-    → BigStep (.ifThenElse t₁ t₂ t₃) v
-  | ifFalse : v.IsValue → BigStep t₁ .falseV → BigStep t₃ v
-    → BigStep (.ifThenElse t₁ t₂ t₃) v
-  | succ : v.IsNumericValue → BigStep t₁ v → BigStep (.succ t₁) (.succ v)
-  | predZero : BigStep t₁ .zero → BigStep (.pred t₁) .zero
-  | predSucc : v.IsNumericValue → BigStep t₁ (.succ v) → BigStep (.pred t₁) v
-  | isZeroZero : BigStep t₁ .zero → BigStep (.isZero t₁) .trueV
-  | isZeroSucc : v.IsNumericValue → BigStep t₁ (.succ v) → BigStep (.isZero t₁) .falseV
+namespace Term
+  inductive BigStep : Term → Term → Prop where
+    | value : v.IsValue → BigStep v v
+    | ifTrue : v.IsValue → BigStep t₁ .trueV → BigStep t₂ v
+      → BigStep (.ifThenElse t₁ t₂ t₃) v
+    | ifFalse : v.IsValue → BigStep t₁ .falseV → BigStep t₃ v
+      → BigStep (.ifThenElse t₁ t₂ t₃) v
+    | succ : v.IsNumericValue → BigStep t₁ v → BigStep (.succ t₁) (.succ v)
+    | predZero : BigStep t₁ .zero → BigStep (.pred t₁) .zero
+    | predSucc : v.IsNumericValue → BigStep t₁ (.succ v) → BigStep (.pred t₁) v
+    | isZeroZero : BigStep t₁ .zero → BigStep (.isZero t₁) .trueV
+    | isZeroSucc : v.IsNumericValue → BigStep t₁ (.succ v) → BigStep (.isZero t₁) .falseV
 
-lemma smallStep_preserves_bigStep : v.IsValue → t ~> t' → BigStep t' v → BigStep t v := by
-  intro v_value t_st_t' t'_bigst_v
-  induction t' generalizing t v <;>
-    grind [BigStep, SmallStep, Term.IsValue, Term.IsNumericValue]
+  lemma smallStep_preserves_bigStep : v.IsValue → t ~> t' → BigStep t' v → BigStep t v := by
+    intro v_value t_st_t' t'_bigst_v
+    induction t' generalizing t v <;>
+      grind [BigStep, SmallStep, Term.IsValue, Term.IsNumericValue]
 
-lemma bigStep_of_smallSteps : v.IsValue → t ~>* v → BigStep t v := by
-  intro v_value t_sts_v
-  induction t_sts_v <;> grind [BigStep, smallStep_preserves_bigStep]
+  lemma bigStep_of_smallSteps : v.IsValue → t ~>* v → BigStep t v := by
+    intro v_value t_sts_v
+    induction t_sts_v <;> grind [BigStep, smallStep_preserves_bigStep]
 
-lemma smallSteps_of_bigStep : v.IsValue → BigStep t v → t ~>* v := by
-  intro v_value t_bigst_v
-  induction t_bigst_v
-  case value => constructor
-  case ifTrue v_value t₁_bst_trueV t₂_bst_v ih_trueV ih_v =>
-    rename_i t₁ t₂ v t₃ _
-    let t₁_sts_trueV := ih_trueV (by constructor)
-    let t₂_sts_v := ih_v v_value
-    let sts₁ : t₁.ifThenElse t₂ t₃ ~>* .ifThenElse .trueV t₂ t₃ := ReflTransGen'.lift
-      (Term.ifThenElse · t₂ t₃) SmallStep.If t₁_sts_trueV
-    let sts₂ : t₁.ifThenElse t₂ t₃ ~>* t₂ := ReflTransGen'.trans' sts₁ .IfTrue
-    exact ReflTransGen'.trans sts₂ t₂_sts_v
-  case ifFalse v_value t₁_bigst_falseV t₂_bst_v ih_falseV ih_v =>
-    rename_i t₁ t₂ v t₃ _
-    let t₁_sts_falseV := ih_falseV (by constructor)
-    let t₂_sts_v := ih_v v_value
-    let sts₁ : t₁.ifThenElse t₃ t₂ ~>* .ifThenElse .falseV t₃ t₂ := ReflTransGen'.lift
-      (Term.ifThenElse · t₃ t₂) SmallStep.If t₁_sts_falseV
-    let sts₂ : t₁.ifThenElse t₃ t₂ ~>* t₂ := ReflTransGen'.trans' sts₁ .IfFalse
-    exact ReflTransGen'.trans sts₂ t₂_sts_v
-  case succ v_value t_bst_v ih =>
-    apply ReflTransGen'.lift Term.succ SmallStep.Succ
-    apply ih
-    cases v_value
-    rename_i v_nv
-    cases v_nv
-    constructor
-    assumption
-  case predZero t_st_zero ih =>
-    let sts₁ := ReflTransGen'.lift Term.pred SmallStep.Pred
-      (ih (by repeat constructor))
-    apply ReflTransGen'.trans' sts₁
-    constructor
-  case predSucc v_nv t_bst_v_succ ih =>
-    let sts₁ := ReflTransGen'.lift Term.pred SmallStep.Pred
-      (ih (by constructor; constructor; assumption))
-    apply ReflTransGen'.trans' sts₁
-    constructor
-    assumption
-  case isZeroZero t_bst_zero ih =>
-    let sts₁ := ReflTransGen'.lift Term.isZero SmallStep.IsZero
-      (ih (by repeat constructor))
-    apply ReflTransGen'.trans' sts₁
-    constructor
-  case isZeroSucc v_nv t_bst_v_succ ih =>
-    let sts₁ := ReflTransGen'.lift Term.isZero SmallStep.IsZero
-      (ih (by constructor; constructor; assumption))
-    apply ReflTransGen'.trans' sts₁
-    constructor
-    assumption
+  lemma smallSteps_of_bigStep : v.IsValue → BigStep t v → t ~>* v := by
+    intro v_value t_bigst_v
+    induction t_bigst_v
+    case value => constructor
+    case ifTrue v_value t₁_bst_trueV t₂_bst_v ih_trueV ih_v =>
+      rename_i t₁ t₂ v t₃ _
+      let t₁_sts_trueV := ih_trueV (by constructor)
+      let t₂_sts_v := ih_v v_value
+      let sts₁ : t₁.ifThenElse t₂ t₃ ~>* .ifThenElse .trueV t₂ t₃ := ReflTransGen'.lift
+        (Term.ifThenElse · t₂ t₃) SmallStep.If t₁_sts_trueV
+      let sts₂ : t₁.ifThenElse t₂ t₃ ~>* t₂ := ReflTransGen'.trans' sts₁ .IfTrue
+      exact ReflTransGen'.trans sts₂ t₂_sts_v
+    case ifFalse v_value t₁_bigst_falseV t₂_bst_v ih_falseV ih_v =>
+      rename_i t₁ t₂ v t₃ _
+      let t₁_sts_falseV := ih_falseV (by constructor)
+      let t₂_sts_v := ih_v v_value
+      let sts₁ : t₁.ifThenElse t₃ t₂ ~>* .ifThenElse .falseV t₃ t₂ := ReflTransGen'.lift
+        (Term.ifThenElse · t₃ t₂) SmallStep.If t₁_sts_falseV
+      let sts₂ : t₁.ifThenElse t₃ t₂ ~>* t₂ := ReflTransGen'.trans' sts₁ .IfFalse
+      exact ReflTransGen'.trans sts₂ t₂_sts_v
+    case succ v_value t_bst_v ih =>
+      apply ReflTransGen'.lift Term.succ SmallStep.Succ
+      apply ih
+      cases v_value
+      rename_i v_nv
+      cases v_nv
+      constructor
+      assumption
+    case predZero t_st_zero ih =>
+      let sts₁ := ReflTransGen'.lift Term.pred SmallStep.Pred
+        (ih (by repeat constructor))
+      apply ReflTransGen'.trans' sts₁
+      constructor
+    case predSucc v_nv t_bst_v_succ ih =>
+      let sts₁ := ReflTransGen'.lift Term.pred SmallStep.Pred
+        (ih (by constructor; constructor; assumption))
+      apply ReflTransGen'.trans' sts₁
+      constructor
+      assumption
+    case isZeroZero t_bst_zero ih =>
+      let sts₁ := ReflTransGen'.lift Term.isZero SmallStep.IsZero
+        (ih (by repeat constructor))
+      apply ReflTransGen'.trans' sts₁
+      constructor
+    case isZeroSucc v_nv t_bst_v_succ ih =>
+      let sts₁ := ReflTransGen'.lift Term.isZero SmallStep.IsZero
+        (ih (by constructor; constructor; assumption))
+      apply ReflTransGen'.trans' sts₁
+      constructor
+      assumption
 
-theorem bigStep_iff_smallSteps : v.IsValue → (BigStep t v ↔ t ~>* v) := by
-  intro v_value
-  constructor
-  · exact smallSteps_of_bigStep v_value
-  · exact bigStep_of_smallSteps v_value
+  theorem bigStep_iff_smallSteps : v.IsValue → (BigStep t v ↔ t ~>* v) := by
+    intro v_value
+    constructor
+    · exact smallSteps_of_bigStep v_value
+    · exact bigStep_of_smallSteps v_value
+end Term
