TAPLFormalization/01-peano/Semantics.lean
@@ -3,19 +3,21 @@ import Mathlib.Logic.Relation
 import TAPLFormalization.«01-peano».AST
 import TAPLFormalization.«01-peano».Common
 
-inductive SmallStep : Term → Term → Prop where
-  | IfTrue : SmallStep (.ifThenElse .trueV t₂ t₃) t₂
-  | IfFalse : SmallStep (.ifThenElse .falseV t₂ t₃) t₃
-  | If : SmallStep t₁ t₂ → SmallStep (.ifThenElse t₁ a b) (.ifThenElse t₂ a b)
-  | Succ :  SmallStep t₁ t₂ → SmallStep (.succ t₁) (.succ t₂)
-  | PredZero : SmallStep (.pred .zero) .zero
-  | PredSucc : nv.IsNumericValue → SmallStep (.pred (.succ nv)) nv
-  | Pred : SmallStep t₁ t₂ → SmallStep (.pred t₁) (.pred t₂)
-  | IsZeroZero : SmallStep (.isZero .zero) .trueV
-  | IsZeroSucc : nv.IsNumericValue → SmallStep (.isZero (.succ nv)) .falseV
-  | IsZero : SmallStep t₁ t₂ → SmallStep (.isZero t₁) (.isZero t₂)
+namespace Term
+  inductive SmallStep : Term → Term → Prop where
+    | IfTrue : SmallStep (.ifThenElse .trueV t₂ t₃) t₂
+    | IfFalse : SmallStep (.ifThenElse .falseV t₂ t₃) t₃
+    | If : SmallStep t₁ t₂ → SmallStep (.ifThenElse t₁ a b) (.ifThenElse t₂ a b)
+    | Succ :  SmallStep t₁ t₂ → SmallStep (.succ t₁) (.succ t₂)
+    | PredZero : SmallStep (.pred .zero) .zero
+    | PredSucc : nv.IsNumericValue → SmallStep (.pred (.succ nv)) nv
+    | Pred : SmallStep t₁ t₂ → SmallStep (.pred t₁) (.pred t₂)
+    | IsZeroZero : SmallStep (.isZero .zero) .trueV
+    | IsZeroSucc : nv.IsNumericValue → SmallStep (.isZero (.succ nv)) .falseV
+    | IsZero : SmallStep t₁ t₂ → SmallStep (.isZero t₁) (.isZero t₂)
 
-abbrev SmallSteps := ReflTransGen' SmallStep
+  abbrev SmallSteps := ReflTransGen' SmallStep
+end Term
 
-infix:100 "~>" => SmallStep
-infix:100 "~>*" => SmallSteps
+infix:100 "~>" => Term.SmallStep
+infix:100 "~>*" => Term.SmallSteps
